%%%%%%%%%%%%%%%%%%%%%%%%%%%%%% Preamble
\documentclass{article}
\usepackage{amsmath,amssymb,amsthm,fullpage}
\usepackage[a4paper,bindingoffset=0in,left=1in,right=1in,top=1in,
bottom=1in,footskip=0in]{geometry}
\newtheorem*{prop}{Proposition}
%\newcounter{Examplecount}
%\setcounter{Examplecount}{0}
\newenvironment{discussion}{\noindent Discussion.}{}
\setlength{\headheight}{12pt}
\setlength{\headsep}{10pt}
\usepackage{fancyhdr}
\pagestyle{fancy}
\fancyhf{}
\lhead{CS144 HW 2}
\rhead{Matt Lim}
\pagenumbering{gobble}
\usepackage{graphicx}
\graphicspath{ {.} }
\begin{document}

%%%%%%%%%%%%%%%%%%%%%%%%%%%%%% Problem 1
\section*{Problem 1}
\subsection*{(a)}
We'll start with

\[ P(D = k) = \binom{n - 1}{k} p^k (1 - p)^{n - 1 - k} \]

\noindent Let's take the limit now

\[ \lim_{n \rightarrow \infty} P(D = k) = \lim_{n \rightarrow \infty} 
    \binom{n - 1}{k} p^k (1 - p)^{n - 1 - k} \]
Using $\lambda := (n - 1)p$, we have 
\[ \lim_{n \rightarrow \infty} P(D = k) = \lim_{n \rightarrow \infty} 
    \frac{(n - 1)!}{k!(n - 1 - k)!} (\frac{\lambda}{n - 1})^k (1 - \frac{\lambda}{n - 1})^{n - 1 - k} \]

\noindent Let's analyze each of these parts separately, starting with the 
factorial expression.

\[ \frac{(n - 1)!}{k!(n - 1 - k)!} = \frac{(n - 1)((n - 1) - 1)\cdots((n - 1) - k + 1)}{k!} \]
The numerator can be approximated as $(n - 1)^k + E$, where
$E$ represents the terms with powers $k - 1$ or less. As $n \rightarrow \infty$, 
$E$ effectively goes to zero, as the $(n - 1)^k$ term dominates.

\noindent Now let's analyze the second part, $(\frac{\lambda}{n - 1})^k$. We can
see that this doesn't need much simplifying. But notice that the denominator here
will cancel with the numerator we calculated in the first part.

\noindent Finally, let's analyze the third part. We can get the following using the 
approximation $(1 + \frac{x}{n})^n = e^x$ 

\[ \lim_{n \rightarrow \infty} (1 - \frac{\lambda}{n - 1})^{n - 1 - k} \]
\[ = (1 - \frac{\lambda}{n - 1})^{n - 1} (1 - \frac{\lambda}{n - 1})^{-k} \]
\[ = e^{-\lambda} 1^{-k} \]
\[ = e^{-\lambda} \]

\noindent Now we can put everything together.
\[ \lim_{n \rightarrow \infty} P(D = k) = \frac{(n - 1)^k }{k!} (\frac{\lambda}{n - 1})^k
    e^{-\lambda} \]
\[ \lim_{n \rightarrow \infty} P(D = k) = \frac{e^{-\lambda} \lambda^k}{k!} \]

\end{document}
